proof/spec/XMSS.ec
@@ -1,0 +1,115 @@
+pragma Goals : printall.
+
+require import AllCore List RealExp IntDiv Distr DList.
+require (*--*) Subtype. 
+
+from Jasmin require import JModel.
+ 
+require import Types Params Notation Parameters Address Hash Primitives Wots Util.
+
+require import XMSS_Commons.
+
+import OTSKeys Three_NBytes AuthPath.
+import Array8.
+
+module XMSS = {
+    proc sample_randomness () : nbytes * nbytes * nbytes = {
+    var sk_seed, sk_prf, pub_seed : nbytes;
+
+    sk_seed <$ DList.dlist W8.dword n;
+    sk_prf <$ DList.dlist W8.dword n;
+    pub_seed <$ DList.dlist W8.dword n;
+
+    return (sk_seed, sk_prf, pub_seed);
+  }
+
+   proc kg() : xmss_mt_keypair = {
+      var pk : xmss_mt_pk <- witness;
+      var sk : xmss_mt_sk <- witness;
+
+      var sk_seed, sk_prf, pub_seed, root : nbytes <- nseq n W8.zero;
+
+      var address : adrs <- zero_address;
+      address <- set_layer_addr address (d - 1);
+      
+      (sk_seed, sk_prf, pub_seed) <@ sample_randomness();
+
+      sk <- {| idx=W32.zero;
+               sk_seed=sk_seed;
+               sk_prf=sk_prf;
+               pub_seed_sk=pub_seed;
+               sk_root=witness;
+             |};
+
+      (root, address) <@ TreeHash.treehash(sk, 0, h, address);
+
+      sk <- {| idx=W32.zero;
+               sk_seed=sk_seed;
+               sk_prf=sk_prf;
+               pub_seed_sk=pub_seed;
+               sk_root=root;
+             |};
+
+      pk <- {| pk_oid=impl_oid; pk_root=root; pk_pub_seed=pub_seed |};
+
+      return (sk, pk);
+   }
+
+proc sign(sk : xmss_mt_sk, m : msg_t) : sig_t * xmss_mt_sk = {
+    var idx : W32.t;
+    var idx_new : W32.t;
+    var address : adrs;
+    var _R : nbytes;
+    var _M' : nbytes;
+    var ots_sig : wots_signature;
+    var auth : auth_path;
+    var sig : sig_t;
+    var idx_bytes : W8.t list;
+    var idx_nbytes : nbytes;
+    var root : nbytes;
+    var t : three_n_bytes;
+    var sk_prf : nbytes <- sk.`sk_prf;
+    
+    idx_new <- sk.`idx + W32.one;
+    sk <- {| sk with idx=idx_new |};
+    address <- zero_address;
+    
+    idx_bytes <- toByte idx 32;
+
+    _R <@ Hash.prf(sk_prf, idx_bytes);
+
+    idx_nbytes <- toByte idx n;
+    root <- sk.`sk_root;
+    t <- _R ++ root ++ idx_nbytes;
+    _M' <- H_msg t m;
+
+    (ots_sig, auth, address) <@ TreeSig.treesig(_M', sk, idx, address);
+
+sig <- {| sig with r_sigs = [(ots_sig, auth)] |}; (* Sig_MT = Sig_MT || r || Sig_tmp; *)
+  
+    return (sig, sk);
+  }
+
+ proc verify(pk : xmss_mt_pk, m : msg_t, s : sig_t) : bool = {
+    var is_valid : bool;
+    var idx_sig : W32.t <- s.`sig_idx;
+    var idx_bytes : nbytes <- toByte idx_sig n;
+    var node, root, _R, _M': nbytes;    
+    var auth : auth_path;
+    var sig_ots : wots_signature;
+    var _seed : seed <- pk.`pk_pub_seed;
+    var address : adrs <- zero_address;
+    var t : three_n_bytes;
+
+    root <- pk.`pk_root;
+    _R <- s.`r;
+    t <- _R ++ root ++ idx_bytes;
+    _M' <- H_msg t m;
+    
+    node <@ RootFromSig.rootFromSig(idx_sig, sig_ots, auth, _M', _seed, address);
+
+    is_valid <- (node = root);
+
+    return is_valid;
+  }  
+}.
